WIP: max_op

nondeterministic_dataflow/Operator.thy
@@ -203,12 +203,17 @@ abbreviation "safe_choice2 f op1s op2s \<equiv> (if op1s = cempty \<and> op2s = 
   else Choice (cimage (case_prod f) (cproduct op1s op2s)))"
 abbreviation "choice1 op \<equiv> Choice (cimage (\<lambda>_. op) {|()|})"
 abbreviation "choice2 op1 op2 \<equiv> Choice (cimage (\<lambda>b. if b then op1 else op2) (cinsert True (csingle False)))"
+abbreviation "choice3 op1 op2 op3 \<equiv> Choice (cimage (\<lambda>b. case b of None \<Rightarrow> op1 | Some True \<Rightarrow> op2 | Some False \<Rightarrow> op3) (cinsert None (cinsert (Some True) (csingle (Some False)))))"
 abbreviation "safe_read f x \<equiv> (case x of None \<Rightarrow> end_op | Some x \<Rightarrow> f x)"
 
 abbreviation "sound_reads wire buf \<equiv> cfilter (\<lambda> op. case op of Read p f \<Rightarrow> p \<notin> ran wire \<or> buf p \<noteq> [] | _ \<Rightarrow> True)"
 
 abbreviation "ARead i f op \<equiv> Choice (cimage (\<lambda> x. if x then op else Read i f) (cinsert True (csingle False)))"
 lemma ARead_simp[simp]: "ARead i f op = Choice ({| op, Read i f |})"
+  by simp
+
+abbreviation "pull i f \<equiv> Choice (cimage (\<lambda> x. if x then f None else Read i (f o Some)) (cinsert True (csingle False)))"
+lemma pull_simp[simp]: "pull i f = Choice ({| f None, Read i (f o Some) |})"
   by simp
 
 lemma map_op_inj_inv:
@@ -1135,7 +1140,7 @@ proof (induct x rule: converse_rtranclp_induct)
       (auto intro: chain.intros dest: chain_nonempty)
 qed (auto intro: chain.intros)
 
-fun lshift (infixr \<open>@-\<close> 65) where
+fun lshift (infixr \<open>@@-\<close> 65) where
   "lshift [] lys = lys"
 | "lshift (x # xs) lys = LCons x (lshift xs lys)"
 
